'Cleanup' but it's mostly shifting things around

theories/encryption/Hybrid.ec
@@ -21,9 +21,11 @@ type outputA.
 
 module Count = {
   var c : int
+
   proc init () : unit = {
     c <- 0;
   }
+
   proc incr () : unit = {
     c <- c + 1;
   }
@@ -36,6 +38,7 @@ module type Adv = {
 module AdvCount (A : Adv) = {
   proc main() : outputA = {
     var r : outputA;
+
     Count.init();
     r <@ A.main();
     return r;
@@ -49,6 +52,7 @@ module type Orcl = {
 module OrclCount (O : Orcl) = {
   proc orcl(m : input) : output = {
     var r : output;
+
     r <@ O.orcl(m);
     Count.incr();
     return r;
@@ -61,7 +65,7 @@ module OrclCount (O : Orcl) = {
 op q : { int | 0 < q } as q_pos.
 
 module type AdvOrcl (O : Orcl) = {
-  proc main () : outputA
+  include Adv
 }.
 
 module type Orclb = {
@@ -78,24 +82,24 @@ module R (Ob : Orclb) : Orcl = {
   proc orcl = Ob.orclR
 }.
 
-module type AdvOrclb (Ob : Orclb, O : Orcl) = {
-  proc main () : outputA
+module type AdvOrclb (Ob : Orclb) (O : Orcl) = {
+  include Adv
 }.
 
-module Orcln (A : AdvOrcl, O : Orcl) = AdvCount(A(OrclCount(O))).
-
-module Ln(Ob : Orclb, A : AdvOrclb) = Orcln(A(Ob), L(Ob)).
-
-module Rn(Ob : Orclb, A : AdvOrclb) = Orcln(A(Ob), R(Ob)).
+module Orcln (A : AdvOrcl) (O : Orcl) = AdvCount(A(OrclCount(O))).
+module Ln (Ob : Orclb) (A : AdvOrclb) = Orcln(A(Ob), L(Ob)).
+module Rn (Ob : Orclb) (A : AdvOrclb) = Orcln(A(Ob), R(Ob)).
 
 (* Hybrid oracle:
    Use left oracle for queries < l0,
    oracle O for queries = l0, and
    right oracle for queries > l0. *)
-module HybOrcl (Ob : Orclb, O : Orcl) = {
+module HybOrcl (Ob : Orclb) (O : Orcl) = {
   var l, l0 : int
+
   proc orcl(m:input):output = {
     var r : output;
+
     if   (l0 < l) r <@ Ob.orclL(m);
     elif (l0 = l) r <@ O.orcl(m);
     else          r <@ Ob.orclR(m);
@@ -106,14 +110,13 @@ module HybOrcl (Ob : Orclb, O : Orcl) = {
 
 (* Hybrid game: Adversary has access to
    leaks, left, right, and hybrid oracle *)
-module HybGame(A:AdvOrclb, Ob:Orclb, O:Orcl) = {
-  module LR = HybOrcl(Ob,O)
-  module A = A(Ob,LR)
+module HybGame (A:AdvOrclb) (Ob:Orclb) (O:Orcl) = {
   proc main() : outputA = {
     var r : outputA;
+
     HybOrcl.l0 <$ [0..q-1];
     HybOrcl.l  <- 0;
-    r <@ A.main();
+    r <@ A(Ob, HybOrcl(Ob, O)).main();
     return r;
   }
 }.
@@ -121,7 +124,7 @@ module HybGame(A:AdvOrclb, Ob:Orclb, O:Orcl) = {
 clone import Means as M with
   type input <- int,
   type output <- outputA,
-  op d <- [0..q-1].
+    op d <- [0..q-1].
 
 (* -------------------------------------------------------------------- *)
 (* Prove that it is equivalent to consider n or 1 calls to the oracle *)
@@ -130,14 +133,22 @@ section.
   declare module Ob : Orclb    {Count,HybOrcl}.
   declare module A  : AdvOrclb {Count,HybOrcl,Ob}.
 
+  axiom losslessL: islossless Ob.leaks.
+  axiom losslessOb1: islossless Ob.orclL.
+  axiom losslessOb2: islossless Ob.orclR.
+  axiom losslessA (Ob0 <: Orclb {A}) (LR <: Orcl {A}):
+    islossless LR.orcl =>
+    islossless Ob0.leaks => islossless Ob0.orclL => islossless Ob0.orclR =>
+    islossless A(Ob0, LR).main.
+
   (* Hybrid game where index is fixed, not sampled *)
   local module HybGameFixed (O : Orcl) = {
-    module LR = HybOrcl(Ob,O)
-    module A = A(Ob,LR)
     proc work(x : int) : outputA = {
       var r : outputA;
-      HybOrcl.l <- 0; HybOrcl.l0 <- x;
-      r <@ A.main();
+
+      HybOrcl.l <- 0;
+      HybOrcl.l0 <- x;
+      r <@ A(Ob, HybOrcl(Ob, O)).main();
       return r;
     }
   }.
@@ -152,160 +163,171 @@ section.
   proof. by proc true. qed.
 
   local lemma GLB_WL &m (p:glob A -> glob Ob -> int -> outputA -> bool):
-    Pr[Ln(Ob,HybGame(A)).main() @ &m : p (glob A) (glob Ob) HybOrcl.l res /\ Count.c <= 1] =
-    Pr[Rand(HybGameFixed(L(Ob))).main() @ &m : p (glob A) (glob Ob) HybOrcl.l (snd res)].
+      Pr[Ln(Ob,HybGame(A)).main() @ &m : p (glob A) (glob Ob) HybOrcl.l res /\ Count.c <= 1]
+    = Pr[Rand(HybGameFixed(L(Ob))).main() @ &m : p (glob A) (glob Ob) HybOrcl.l (snd res)].
   proof.
-    byequiv (_ : ={glob A, glob Ob} ==>
-                    ={glob A, glob Ob,glob HybOrcl} /\ res{1} = snd res{2} /\
-                    Count.c{1} <= 1) => //;proc.
-    inline{1} HybGame(A, Ob, OrclCount(L(Ob))).main; inline{2} HybGameFixed(L(Ob)).work;wp.
-    call (_: ={glob Ob, glob HybOrcl} /\ Count.c{1} = (HybOrcl.l0{1} < HybOrcl.l{1}) ? 1 : 0).
-      proc;wp.
-      if => //;first by call Oborcl1;skip;progress => //; smt.
-      if => //.
-        inline{1} OrclCount(L(Ob)).orcl Count.incr.
-        by wp;call Oborcl1;wp;skip;progress => //;smt.
-      by call Oborcl2;skip;progress => //; smt.
-      by conseq Obleaks.
-      by conseq Oborcl1.
-      by conseq Oborcl2.
-    swap{1} 1 2;inline{1} Count.init.
-    by wp;rnd;wp;skip;progress => //;smt.
+  byequiv (: ={glob A, glob Ob}
+             ==>    ={glob A, glob Ob,glob HybOrcl}
+                 /\ res{1} = snd res{2}
+                 /\ Count.c{1} <= 1)=> //.
+  proc.
+  inline {1} HybGame(A, Ob, OrclCount(L(Ob))).main.
+  inline {2} HybGameFixed(L(Ob)).work.
+  wp; call (:    ={glob Ob, glob HybOrcl}
+              /\ Count.c{1} = (HybOrcl.l0{1} < HybOrcl.l{1}) ? 1 : 0).
+  + proc; wp.
+    if=> //.
+    + by call Oborcl1; auto=> /#.
+    if=> //.
+    + inline {1} OrclCount(L(Ob)).orcl Count.incr.
+      by wp; call Oborcl1; auto=> /#.
+    by call Oborcl2; auto=> /#.
+  + by conseq Obleaks.
+  + by conseq Oborcl1.
+  + by conseq Oborcl2.
+  swap {1} 1 2; inline {1} Count.init.
+  by auto=> /> l0 /supp_dinter /#.
   qed.
 
   local lemma GRB_WR &m (p:glob A -> glob Ob -> int -> outputA -> bool):
-    Pr[Rn(Ob,HybGame(A)).main() @ &m : p (glob A) (glob Ob) HybOrcl.l res /\ Count.c <= 1] =
-    Pr[Rand(HybGameFixed(R(Ob))).main() @ &m : p (glob A) (glob Ob) HybOrcl.l (snd res)].
+      Pr[Rn(Ob,HybGame(A)).main() @ &m : p (glob A) (glob Ob) HybOrcl.l res /\ Count.c <= 1]
+    = Pr[Rand(HybGameFixed(R(Ob))).main() @ &m : p (glob A) (glob Ob) HybOrcl.l (snd res)].
   proof.
-    byequiv (_ : ={glob A, glob Ob} ==>
-                    ={glob A, glob Ob, glob HybOrcl} /\ res{1} = snd res{2} /\
-                    Count.c{1} <= 1) => //;proc.
-    inline{1} HybGame(A, Ob, OrclCount(R(Ob))).main; inline{2} HybGameFixed(R(Ob)).work;wp.
-    call (_: ={glob Ob, glob HybGame} /\ Count.c{1} = (HybOrcl.l0{1} < HybOrcl.l{1}) ? 1 : 0).
-      proc;wp.
-      if => //;first by call Oborcl1;skip;progress => //; smt.
-      if => //.
-        inline{1} OrclCount(R(Ob)).orcl Count.incr.
-        by wp;call Oborcl2;wp;skip;progress => //;smt.
-      by call Oborcl2;skip;progress => //; smt.
-      by conseq Obleaks.
-      by conseq Oborcl1.
-      by conseq Oborcl2.
-    swap{1} 1 2;inline{1} Count.init.
-    by wp;rnd;wp;skip;progress => //;smt.
+  byequiv (: ={glob A, glob Ob}
+             ==>    ={glob A, glob Ob, glob HybOrcl}
+                 /\ res{1} = snd res{2}
+                 /\ Count.c{1} <= 1)=> //.
+  proc.
+  inline {1} HybGame(A, Ob, OrclCount(R(Ob))).main.
+  inline {2} HybGameFixed(R(Ob)).work.
+  wp; call (:    ={glob Ob, glob HybGame}
+              /\ Count.c{1} = (HybOrcl.l0{1} < HybOrcl.l{1}) ? 1 : 0).
+  + proc; wp.
+    if=> //.
+    + by call Oborcl1; auto=> /#.
+    if=> //.
+    + inline {1} OrclCount(R(Ob)).orcl Count.incr.
+      by wp; call Oborcl2; auto=> /#.
+    by call Oborcl2; auto=> /#.
+  + by conseq Obleaks.
+  + by conseq Oborcl1.
+  + by conseq Oborcl2.
+  swap {1} 1 2; inline {1} Count.init.
+  by auto=> /> l0 /supp_dinter /#.
   qed.
 
-  axiom losslessL: islossless Ob.leaks.
-  axiom losslessOb1: islossless Ob.orclL.
-  axiom losslessOb2: islossless Ob.orclR.
-  axiom losslessA (Ob0 <: Orclb{A}) (LR <: Orcl{A}):
-    islossless LR.orcl =>
-    islossless Ob0.leaks => islossless Ob0.orclL => islossless Ob0.orclR =>
-    islossless A(Ob0, LR).main.
-
   local lemma WL0_GLA &m (p:glob A -> glob Ob -> int -> outputA -> bool):
-    Pr[HybGameFixed(L(Ob)).work(0) @ &m : p (glob A) (glob Ob) HybOrcl.l res /\ HybOrcl.l <= q] =
-    Pr[Ln(Ob,A).main() @ &m : p (glob A) (glob Ob) Count.c res /\ Count.c <= q ].
+      Pr[HybGameFixed(L(Ob)).work(0) @ &m : p (glob A) (glob Ob) HybOrcl.l res /\ HybOrcl.l <= q]
+    = Pr[Ln(Ob,A).main() @ &m : p (glob A) (glob Ob) Count.c res /\ Count.c <= q ].
   proof.
-    byequiv (_ : ={glob A, glob Ob} /\ x{1}=0 ==>
-                    (HybOrcl.l{1} <= q) = (Count.c{2} <= q) /\
-                    (Count.c{2} <= q =>
-                      ={glob A, glob Ob,res} /\ HybOrcl.l{1} = Count.c{2})) => //;
-     [proc | smt].
-    call (_: q < Count.c,
-             ={glob Ob} /\ HybOrcl.l0{1} = 0 /\ HybOrcl.l{1} = Count.c{2} /\ 0 <= HybOrcl.l{1},
-             HybOrcl.l0{1} = 0 /\ q < HybOrcl.l{1}).
-      by apply losslessA.
-      proc;inline{2} Count.incr;wp.
-      if{1};first by call Oborcl1;wp;skip;progress => //;smt.
-      rcondt{1} 1; first by move=> &m0;skip;smt.
-      by wp;call Oborcl1;wp;skip;progress => //;smt.
-      move=> &m2 _;proc.
-      rcondt 1; first by skip;smt.
-      by wp;call losslessOb1;skip;smt.
-      by move=> &m1;proc;inline Count.incr;wp;call losslessOb1;wp;skip;smt.
-      by conseq Obleaks.
-      move=> &m2 _;conseq losslessL.
-      move=> &m1; conseq losslessL.
-
-      by conseq Oborcl1.
-      move=> &m2 _;conseq losslessOb1.
-      move=> &m1; conseq losslessOb1.
-
-      by conseq Oborcl2.
-      move=> &m2 _;conseq losslessOb2.
-      move=> &m1; conseq losslessOb2.
-
-    by inline{2} Count.init;wp;skip;smt.
+  byequiv (:    ={glob A, glob Ob}
+             /\ x{1} = 0
+             ==>    (HybOrcl.l{1} <= q) = (Count.c{2} <= q)
+                 /\ (   Count.c{2} <= q
+                     =>    ={glob A, glob Ob,res}
+                        /\ HybOrcl.l{1} = Count.c{2}))=> // [|/#].
+  proc.
+  call (: q < Count.c
+        ,    ={glob Ob}
+          /\ HybOrcl.l0{1} = 0
+          /\ HybOrcl.l{1} = Count.c{2}
+          /\ 0 <= HybOrcl.l{1}
+        ,    HybOrcl.l0{1} = 0
+          /\ q < HybOrcl.l{1}).
+  + by apply losslessA.
+  + proc; inline {2} Count.incr; wp.
+    if{1}.
+    + by call Oborcl1; auto=> /#.
+    rcondt {1} 1; first by auto=> /#.
+    by wp; call Oborcl1; auto=> /#.
+  + move=> _ _; proc.
+    rcondt 1; first by auto; smt(q_pos).
+    by wp; call losslessOb1; auto=> /#.
+  + by move=> &1; proc; inline Count.incr; wp; call losslessOb1; auto=> /#.
+  + by conseq Obleaks.
+  + by move=> _ _; conseq losslessL.
+  + by move=> &1; conseq losslessL.
+  + by conseq Oborcl1.
+  + by move=> _ _; conseq losslessOb1.
+  + by move=> &1; conseq losslessOb1.
+  + by conseq Oborcl2.
+  + by move=> _ _; conseq losslessOb2.
+  + by move=> &1; conseq losslessOb2.
+  by inline {2} Count.init; auto=> /#.
   qed.
 
   local lemma WRq_GRA &m (p:glob A -> glob Ob -> int -> outputA -> bool):
-    Pr[HybGameFixed(R(Ob)).work((q-1)) @ &m :  p (glob A) (glob Ob) HybOrcl.l res /\ HybOrcl.l <= q] =
-    Pr[Rn(Ob,A).main() @ &m :  p (glob A) (glob Ob) Count.c res /\ Count.c <= q ].
+      Pr[HybGameFixed(R(Ob)).work((q-1)) @ &m :  p (glob A) (glob Ob) HybOrcl.l res /\ HybOrcl.l <= q]
+    = Pr[Rn(Ob,A).main() @ &m :  p (glob A) (glob Ob) Count.c res /\ Count.c <= q ].
   proof.
-    byequiv (_ : ={glob A, glob Ob} /\ x{1}=q-1 ==>
-                    (HybOrcl.l{1} <= q) = (Count.c{2} <= q) /\
-                    (Count.c{2} <= q =>
-                      ={glob A, glob Ob, res} /\ HybOrcl.l{1} = Count.c{2})) => //;
-    [proc | smt].
-    call (_: q < Count.c,
-             ={glob Ob} /\ HybOrcl.l0{1} = q-1 /\ HybOrcl.l{1} = Count.c{2} /\ 0 <= HybOrcl.l{1},
-             HybOrcl.l0{1} = q-1 /\ q < HybOrcl.l{1}).
-      by apply losslessA.
-
-      proc;inline{2} Count.incr;wp.
-      if{1};first by call{1} losslessOb1;call{2} losslessOb2;wp;skip; smt.
-      if{1};
-        first by wp;call Oborcl2;wp;skip;progress => //;smt.
-      by call Oborcl2;wp;skip;progress => //;smt.
-      move=> &m2 _;proc.
-      rcondt 1; first by skip;smt.
-      by wp;call losslessOb1;skip; smt.
-      move=> &m1;proc;inline Count.incr;wp;call losslessOb2;wp;skip;smt.
-
-      by conseq Obleaks.
-      move=> &m2 _;conseq losslessL.
-      move=> &m1; conseq losslessL.
-
-      by conseq Oborcl1.
-      move=> &m2 _;conseq losslessOb1.
-      move=> &m1; conseq losslessOb1.
-
-      by conseq Oborcl2.
-      move=> &m2 _;conseq losslessOb2.
-      move=> &m1; conseq losslessOb2.
-
-    by inline{2} Count.init;wp;skip;smt.
+  byequiv (:    ={glob A, glob Ob}
+             /\ x{1} = q - 1
+             ==>    (HybOrcl.l{1} <= q) = (Count.c{2} <= q)
+                 /\ (   Count.c{2} <= q
+                     =>    ={glob A, glob Ob, res}
+                        /\ HybOrcl.l{1} = Count.c{2}))=> // [|/#].
+  proc.
+  call (: q < Count.c
+        ,    ={glob Ob}
+          /\ HybOrcl.l0{1} = q - 1
+          /\ HybOrcl.l{1} = Count.c{2}
+          /\ 0 <= HybOrcl.l{1}
+        ,    HybOrcl.l0{1} = q - 1
+          /\ q < HybOrcl.l{1}).
+  + by apply losslessA.
+  + proc; inline {2} Count.incr; wp.
+    if{1}.
+    + by call {1} losslessOb1; call {2} losslessOb2; auto=> /#.
+    if{1}.
+    + by wp; call Oborcl2; auto=> /#.
+    by call Oborcl2; auto=> /#.
+  + move=> _ _; proc.
+    rcondt 1; first by auto=> /#.
+    by wp; call losslessOb1; auto=> /#.
+  + by move=> &1; proc; inline Count.incr; wp; call losslessOb2; auto=> /#.
+  + by conseq Obleaks.
+  + by move=> _ _; conseq losslessL.
+  + by move=> &1; conseq losslessL.
+  + by conseq Oborcl1.
+  + by move=> _ _; conseq losslessOb1.
+  + by move=> &1; conseq losslessOb1.
+  + by conseq Oborcl2.
+  + by move=> _ _; conseq losslessOb2.
+  + by move=> &1; conseq losslessOb2.
+  by inline {2} Count.init; auto=> /#.
   qed.
 
   local lemma WLR_shift &m v (p:glob A -> glob Ob -> int -> outputA -> bool):
-    1 <= v <= q-1 =>
-    Pr[HybGameFixed(L(Ob)).work(v) @ &m: p (glob A) (glob Ob) HybOrcl.l res] =
-    Pr[HybGameFixed(R(Ob)).work((v-1)) @ &m : p (glob A) (glob Ob) HybOrcl.l res].
+       1 <= v <= q - 1
+    =>   Pr[HybGameFixed(L(Ob)).work(v) @ &m: p (glob A) (glob Ob) HybOrcl.l res]
+       = Pr[HybGameFixed(R(Ob)).work((v-1)) @ &m : p (glob A) (glob Ob) HybOrcl.l res].
   proof.
-    move=> Hv;byequiv (_: ={glob A,glob Ob} /\ x{1} = v /\ x{2} = v-1 ==>
-                             ={glob A,glob Ob, HybOrcl.l, res}) => //.
-    proc.
-    call (_: ={glob Ob, HybOrcl.l} /\ HybOrcl.l0{1} = v /\ HybOrcl.l0{2} = v-1).
-      proc.
-      if{1}; first by rcondt{2} 1;[move=> &m0;skip;smt | wp;call Oborcl1].
-      if{1};first by rcondt{2} 1;
-       [move=> &m0;skip;smt | wp;call Oborcl1;wp].
-      rcondf{2} 1;first by move=> &m0;skip;smt.
-      by if{2};wp;call Oborcl2;wp.
-      by conseq Obleaks.
-      by conseq Oborcl1.
-      by conseq Oborcl2.
-    by wp.
+  move=> Hv.
+  byequiv (:    ={glob A, glob Ob}
+             /\ x{1} = v
+             /\ x{2} = v - 1
+             ==>    ={glob A, glob Ob, HybOrcl.l, res})=> //.
+  proc.
+  call (: ={glob Ob, HybOrcl.l} /\ HybOrcl.l0{1} = v /\ HybOrcl.l0{2} = v - 1).
+  + proc.
+    if{1}.
+    + by rcondt{2} 1; [ | wp; call Oborcl1 ]; auto=> /#.
+    if{1}.
+    + by rcondt{2} 1; [ | wp; call Oborcl1 ]; auto=> /#.
+    rcondf{2} 1; first by auto=> /#.
+    by if{2}; wp; call Oborcl2; wp.
+  + by conseq Obleaks.
+  + by conseq Oborcl1.
+  + by conseq Oborcl2.
+  by wp.
   qed.
 
   lemma Hybrid &m (p:glob A -> glob Ob -> int -> outputA -> bool):
     let p' = fun ga ge l r, p ga ge l r /\ l <= q in
-    Pr[Ln(Ob,HybGame(A)).main() @ &m : p' (glob A) (glob Ob) HybOrcl.l res /\ Count.c <= 1] -
-      Pr[Rn(Ob,HybGame(A)).main() @ &m : p' (glob A) (glob Ob) HybOrcl.l res /\ Count.c <= 1] =
-    1%r/q%r * (
-      Pr[Ln(Ob,A).main() @ &m : p' (glob A) (glob Ob) Count.c res] -
-        Pr[Rn(Ob,A).main() @ &m : p' (glob A) (glob Ob) Count.c res]).
+        Pr[Ln(Ob,HybGame(A)).main() @ &m : p' (glob A) (glob Ob) HybOrcl.l res /\ Count.c <= 1]
+      - Pr[Rn(Ob,HybGame(A)).main() @ &m : p' (glob A) (glob Ob) HybOrcl.l res /\ Count.c <= 1]
+    = 1%r/q%r * (  Pr[Ln(Ob,A).main() @ &m : p' (glob A) (glob Ob) Count.c res]
+                 - Pr[Rn(Ob,A).main() @ &m : p' (glob A) (glob Ob) Count.c res]).
   proof.
   move=> p';rewrite (GLB_WL &m p') (GRB_WR &m p').
   simplify p'; rewrite -(WL0_GLA &m p) -(WRq_GRA &m p).
@@ -347,7 +369,6 @@ section.
   + by rewrite iter0.
   by rewrite iterS.
   qed.
-
 end section.
 
 (* -------------------------------------------------------------------- *)
@@ -356,13 +377,22 @@ section.
   declare module Ob : Orclb    {Count,HybOrcl}.
   declare module A  : AdvOrclb {Count,HybOrcl,Ob}.
 
-  axiom A_call : forall (O<:Orcl{Count,A}), hoare [ Orcln(A(Ob), O).main : true ==> Count.c <= q ].
+  axiom A_call : forall (O <: Orcl{Count,A}), hoare [ Orcln(A(Ob), O).main : true ==> Count.c <= q ].
+
+  axiom losslessL: islossless Ob.leaks.
+  axiom losslessOb1: islossless Ob.orclL.
+  axiom losslessOb2: islossless Ob.orclR.
+  axiom losslessA (Ob0 <: Orclb{A}) (LR <: Orcl{A}):
+    islossless LR.orcl =>
+    islossless Ob0.leaks => islossless Ob0.orclL => islossless Ob0.orclR =>
+    islossless A(Ob0, LR).main.
 
   local module Al = Orcln(A(Ob),HybOrcl(Ob,L(Ob))).
 
   local module Bl = {
     proc main() : outputA = {
       var r : outputA;
+
       HybOrcl.l0 <$ [0..q-1];
       HybOrcl.l  <- 0;
       r <@ Al.main();
@@ -375,6 +405,7 @@ section.
   local module Br = {
     proc main() : outputA = {
       var r : outputA;
+
       HybOrcl.l0 <$ [0..q-1];
       HybOrcl.l  <- 0;
       r <@ Ar.main();
@@ -386,117 +417,125 @@ section.
      ={glob A, glob Ob} ==>
      ={glob A, glob Ob, glob HybOrcl, res} /\ Count.c{2} = HybOrcl.l{2} /\ Count.c{2} <= q.
   proof.
-    conseq [-frame] (_:  ={glob A, glob Ob} ==>  ={glob A, glob Ob, glob HybOrcl, res}) _
-           (_:true ==> Count.c = HybOrcl.l /\ Count.c <= q).
-     conseq [-frame] (_:true ==> Count.c = HybOrcl.l) (_: true ==> Count.c <= q).
-       proc; call (A_call (<:HybOrcl(Ob,L(Ob)))) => //.
-     proc;inline *;wp;call (_ : Count.c = HybOrcl.l).
-     proc;inline *;wp; by conseq (_: _ ==> true) => //.
-     conseq (_: _ ==> true) => //. conseq (_: _ ==> true) => //. conseq (_: _ ==> true) => //.
-     by wp.
-    proc;inline Al.main;wp. call (_: ={glob Ob, glob HybOrcl}).
-    proc;inline *;wp. sp;if => //. call (_:true) => //.
-      if => //. wp;call (_:true) => //. wp=> //. call (_:true) => //.
-    proc (={glob HybOrcl}) => //. proc (={glob HybOrcl}) => //. proc (={glob HybOrcl}) => //.
-    inline *;wp;rnd => //.
+  conseq (:  ={glob A, glob Ob} ==> ={glob A, glob Ob, glob HybOrcl, res})
+         _
+         (: true ==> Count.c = HybOrcl.l /\ Count.c <= q).
+  + conseq (: true ==> Count.c = HybOrcl.l) (: true ==> Count.c <= q).
+    + by proc; call (A_call (<: HybOrcl(Ob,L(Ob))))=> //.
+    proc; inline *; wp; call (: Count.c = HybOrcl.l).
+    + by proc; inline *; wp; conseq (: _ ==> true).
+    + by conseq (: _ ==> true).
+    + by conseq (: _ ==> true).
+    + by conseq (: _ ==> true).
+    by wp.
+  proc; inline Al.main; wp; call (: ={glob Ob, glob HybOrcl}).
+  + proc; inline *; wp; sp; if=> //.
+    + by call (: true).
+    by if=> //; wp; call (: true).
+  + by proc (={glob HybOrcl}).
+  + by proc (={glob HybOrcl}).
+  + by proc (={glob HybOrcl}).
+  by inline *; auto.
   qed.
 
   local equiv B_Br : HybGame(A,Ob,R(Ob)).main ~ Br.main :
      ={glob A, glob Ob} ==>
      ={glob A, glob Ob, glob HybOrcl, res} /\ Count.c{2} = HybOrcl.l{2} /\ Count.c{2} <= q.
   proof.
-    conseq [-frame] (_:  ={glob A, glob Ob} ==>  ={glob A, glob Ob, glob HybOrcl, res}) _
-           (_:true ==> Count.c = HybOrcl.l /\ Count.c <= q).
-     conseq [-frame] (_:true ==> Count.c = HybOrcl.l) (_: true ==> Count.c <= q).
-       proc; call (A_call (<:HybOrcl(Ob,R(Ob)))) => //.
-     proc;inline *;wp;call (_ : Count.c = HybOrcl.l).
-     proc;inline *;wp; by conseq (_: _ ==> true) => //.
-     conseq (_: _ ==> true) => //. conseq (_: _ ==> true) => //. conseq (_: _ ==> true) => //.
-     by wp.
-    proc;inline Ar.main;wp. call (_: ={glob Ob, glob HybOrcl}).
-    proc;inline *;wp. sp;if => //. call (_:true) => //.
-      if => //. wp;call (_:true) => //. wp=> //. call (_:true) => //.
-    proc (={glob HybOrcl}) => //. proc (={glob HybOrcl}) => //. proc (={glob HybOrcl}) => //.
-    inline *;wp;rnd => //.
+  conseq (: ={glob A, glob Ob} ==> ={glob A, glob Ob, glob HybOrcl, res})
+         _
+         (: true ==> Count.c = HybOrcl.l /\ Count.c <= q).
+  + conseq (: true ==> Count.c = HybOrcl.l) (: true ==> Count.c <= q).
+    + by proc; call (A_call (<: HybOrcl(Ob,R(Ob)))).
+    proc; inline *; wp; call (: Count.c = HybOrcl.l).
+    + by proc; inline *; wp; conseq (: _ ==> true).
+    + by conseq (: _ ==> true).
+    + by conseq (: _ ==> true).
+    + by conseq (: _ ==> true).
+    by wp.
+  proc; inline Ar.main; wp; call (: ={glob Ob, glob HybOrcl}).
+  + proc; inline *; wp; sp; if=> //.
+    + by call (: true).
+    by if=> //; wp; call (: true).
+  + by proc (={glob HybOrcl}).
+  + by proc (={glob HybOrcl}).
+  + by proc (={glob HybOrcl}).
+  by inline *; auto.
   qed.
 
   local lemma Pr_Bl &m (p:glob A -> glob Ob -> int -> outputA -> bool):
-     Pr[HybGame(A,Ob,L(Ob)).main() @ &m : p (glob A) (glob Ob) HybOrcl.l res] =
-     Pr[HybGame(A,Ob,L(Ob)).main() @ &m : p (glob A) (glob Ob) HybOrcl.l res /\ HybOrcl.l <= q].
+       Pr[HybGame(A,Ob,L(Ob)).main() @ &m : p (glob A) (glob Ob) HybOrcl.l res]
+     = Pr[HybGame(A,Ob,L(Ob)).main() @ &m : p (glob A) (glob Ob) HybOrcl.l res /\ HybOrcl.l <= q].
   proof.
-    have -> :
-       Pr[HybGame(A,Ob,L(Ob)).main() @ &m : p (glob A) (glob Ob) HybOrcl.l res] =
-       Pr[Bl.main() @ &m : p (glob A) (glob Ob) HybOrcl.l res /\ HybOrcl.l <= q].
-      byequiv B_Bl => //.
-    apply eq_sym.  byequiv B_Bl => //.
+  have ->:
+      Pr[HybGame(A,Ob,L(Ob)).main() @ &m : p (glob A) (glob Ob) HybOrcl.l res]
+    = Pr[Bl.main() @ &m : p (glob A) (glob Ob) HybOrcl.l res /\ HybOrcl.l <= q].
+  + by byequiv B_Bl.
+  apply eq_sym.
+  by byequiv B_Bl.
   qed.
 
   local lemma Pr_Br &m (p:glob A -> glob Ob -> int -> outputA -> bool):
-     Pr[HybGame(A,Ob,R(Ob)).main() @ &m : p (glob A) (glob Ob) HybOrcl.l res] =
-     Pr[HybGame(A,Ob,R(Ob)).main() @ &m : p (glob A) (glob Ob) HybOrcl.l res /\ HybOrcl.l <= q].
+       Pr[HybGame(A,Ob,R(Ob)).main() @ &m : p (glob A) (glob Ob) HybOrcl.l res]
+     = Pr[HybGame(A,Ob,R(Ob)).main() @ &m : p (glob A) (glob Ob) HybOrcl.l res /\ HybOrcl.l <= q].
   proof.
-    have -> :
-       Pr[HybGame(A,Ob,R(Ob)).main() @ &m : p (glob A) (glob Ob) HybOrcl.l res] =
-       Pr[Br.main() @ &m : p (glob A) (glob Ob) HybOrcl.l res /\ HybOrcl.l <= q].
-      byequiv B_Br => //.
-    apply eq_sym.  byequiv B_Br => //.
+  have ->:
+      Pr[HybGame(A,Ob,R(Ob)).main() @ &m : p (glob A) (glob Ob) HybOrcl.l res]
+    = Pr[Br.main() @ &m : p (glob A) (glob Ob) HybOrcl.l res /\ HybOrcl.l <= q].
+  + by byequiv B_Br.
+  apply eq_sym.
+  by byequiv B_Br.
   qed.
 
-  axiom losslessL: islossless Ob.leaks.
-  axiom losslessOb1: islossless Ob.orclL.
-  axiom losslessOb2: islossless Ob.orclR.
-  axiom losslessA (Ob0 <: Orclb{A}) (LR <: Orcl{A}):
-    islossless LR.orcl =>
-    islossless Ob0.leaks => islossless Ob0.orclL => islossless Ob0.orclR =>
-    islossless A(Ob0, LR).main.
-
   lemma Hybrid_restr &m (p:glob A -> glob Ob -> int -> outputA -> bool):
-      Pr[HybGame(A,Ob,L(Ob)).main() @ &m : p (glob A) (glob Ob) HybOrcl.l res] -
-      Pr[HybGame(A,Ob,R(Ob)).main() @ &m : p (glob A) (glob Ob) HybOrcl.l res] =
-      1%r/q%r * (
-         Pr[Ln(Ob,A).main() @ &m : p (glob A) (glob Ob) Count.c res] -
-         Pr[Rn(Ob,A).main() @ &m : p (glob A) (glob Ob) Count.c res]).
-   proof.
-     pose p' := fun ga ge l r, p ga ge l r /\ l <= q.
-     have -> : Pr[Ln(Ob,A).main() @ &m : p  (glob A) (glob Ob) Count.c res] =
-              Pr[Ln(Ob,A).main() @ &m : p' (glob A) (glob Ob) Count.c res].
-       byequiv (_ : ={glob A, glob Ob} ==> ={glob A, glob Ob, Count.c, res} /\ Count.c{1} <= q) => //;
-         last by rewrite /p'.
-       conseq [-frame] (_:  ={glob A, glob Ob} ==> ={glob A, glob Ob, Count.c, res}) (_ : true ==> Count.c <= q);
-         last by sim;  proc (={Count.c}).
-       apply (A_call (<:L(Ob))).
-     have -> : Pr[Rn(Ob,A).main() @ &m : p  (glob A) (glob Ob) Count.c res] =
-              Pr[Rn(Ob,A).main() @ &m : p' (glob A) (glob Ob) Count.c res].
-       byequiv (_ : ={glob A, glob Ob} ==> ={glob A, glob Ob, Count.c, res} /\ Count.c{1} <= q) => //;
-         last by rewrite /p'.
-       conseq [-frame] (_:  ={glob A, glob Ob} ==> ={glob A, glob Ob, Count.c, res}) (_ : true ==> Count.c <= q);
-         last by sim;  proc (={Count.c}).
-       apply (A_call (<:R(Ob))).
-     rewrite (Pr_Bl &m p) (Pr_Br &m p).
-     have := Hybrid Ob A _ _ _ _ &m p.
-      apply losslessL. apply losslessOb1. apply losslessOb2. apply losslessA.
-     move=> /= H. rewrite /p' -H.
-     congr; last congr.
-     byequiv (_ : ={glob A, glob Ob} ==> ={glob A, glob Ob, glob HybOrcl, res} /\ Count.c{2} <= 1) => //.
-       proc;inline *;wp.
-       call (_ : ={glob Ob, glob HybOrcl} /\ (if HybOrcl.l <= HybOrcl.l0 then Count.c = 0 else Count.c =1){2}).
-        proc. inline *;wp.
-        if => //. call (_: ={glob HybOrcl});auto; smt.
-        if => //. wp;call (_: ={glob HybOrcl});auto; smt. call (_: ={glob HybOrcl});auto; smt.
-       conseq (_: _ ==> ={res,glob Ob}) => //. sim.
-       conseq (_: _ ==> ={res,glob Ob}) => //. sim.
-       conseq (_: _ ==> ={res,glob Ob}) => //. sim.
-       auto;progress;smt.
-     byequiv (_ : ={glob A, glob Ob} ==> ={glob A, glob Ob, glob HybOrcl, res} /\ Count.c{2} <= 1) => //.
-       proc;inline *;wp.
-       call (_ : ={glob Ob, glob HybOrcl} /\ (if HybOrcl.l <= HybOrcl.l0 then Count.c = 0 else Count.c =1){2}).
-        proc. inline *;wp.
-        if => //. call (_: ={glob HybOrcl});auto; smt.
-        if => //. wp;call (_: ={glob HybOrcl});auto; smt. call (_: ={glob HybOrcl});auto; smt.
-       conseq (_: _ ==> ={res,glob Ob}) => //. sim.
-       conseq (_: _ ==> ={res,glob Ob}) => //. sim.
-       conseq (_: _ ==> ={res,glob Ob}) => //. sim.
-       auto;progress;smt.
-    qed.
-
+        Pr[HybGame(A,Ob,L(Ob)).main() @ &m : p (glob A) (glob Ob) HybOrcl.l res]
+      - Pr[HybGame(A,Ob,R(Ob)).main() @ &m : p (glob A) (glob Ob) HybOrcl.l res]
+    = 1%r/q%r * (  Pr[Ln(Ob,A).main() @ &m : p (glob A) (glob Ob) Count.c res]
+                 - Pr[Rn(Ob,A).main() @ &m : p (glob A) (glob Ob) Count.c res]).
+  proof.
+  pose p' := fun ga ge l r, p ga ge l r /\ l <= q.
+  have ->:   Pr[Ln(Ob,A).main() @ &m : p  (glob A) (glob Ob) Count.c res]
+           = Pr[Ln(Ob,A).main() @ &m : p' (glob A) (glob Ob) Count.c res].
+  + byequiv (: ={glob A, glob Ob} ==> ={glob A, glob Ob, Count.c, res} /\ Count.c{1} <= q)=> [| |@/p'] //=.
+    conseq (: ={glob A, glob Ob} ==> ={glob A, glob Ob, Count.c, res}) (: true ==> Count.c <= q).
+    + exact/(A_call (<: L(Ob))).
+    by sim.
+  have ->:   Pr[Rn(Ob,A).main() @ &m : p  (glob A) (glob Ob) Count.c res]
+           = Pr[Rn(Ob,A).main() @ &m : p' (glob A) (glob Ob) Count.c res].
+  + byequiv (: ={glob A, glob Ob} ==> ={glob A, glob Ob, Count.c, res} /\ Count.c{1} <= q)=> [| |@/p'] //=.
+    conseq (: ={glob A, glob Ob} ==> ={glob A, glob Ob, Count.c, res}) (: true ==> Count.c <= q).
+    + exact/(A_call (<: R(Ob))).
+    by sim.
+  rewrite (Pr_Bl &m p) (Pr_Br &m p).
+  have /= H := Hybrid Ob A losslessL losslessOb1 losslessOb2 losslessA &m p.
+  rewrite /p' -H.
+  congr.
+  + byequiv (: ={glob A, glob Ob} ==> ={glob A, glob Ob, glob HybOrcl, res} /\ Count.c{2} <= 1)=> //.
+    proc; inline *; wp.
+    call (: ={glob Ob, glob HybOrcl} /\ (if HybOrcl.l <= HybOrcl.l0 then Count.c = 0 else Count.c =1){2}).
+    + proc; inline *; wp.
+      if=> //.
+      + by call (: ={glob HybOrcl}); auto=> /#.
+      if=> //.
+      + by wp; call (: ={glob HybOrcl}); auto=> /#.
+      by call (: ={glob HybOrcl}); auto=> /#.
+    + by conseq (: _ ==> ={res,glob Ob})=> //; sim.
+    + by conseq (: _ ==> ={res,glob Ob})=> //; sim.
+    + by conseq (: _ ==> ={res,glob Ob})=> //; sim.
+    by auto=> /> l0 /supp_dinter /#.
+  congr.
+  byequiv (: ={glob A, glob Ob} ==> ={glob A, glob Ob, glob HybOrcl, res} /\ Count.c{2} <= 1)=> //.
+  proc; inline *; wp.
+  call (: ={glob Ob, glob HybOrcl} /\ (if HybOrcl.l <= HybOrcl.l0 then Count.c = 0 else Count.c =1){2}).
+  + proc; inline *; wp.
+    if=> //.
+    + by call (: ={glob HybOrcl}); auto=> /#.
+    if=> //.
+    + by wp; call (: ={glob HybOrcl}); auto=> /#.
+    by call (: ={glob HybOrcl}); auto=> /#.
+  + by conseq (: _ ==> ={res, glob Ob})=> //; sim.
+  + by conseq (: _ ==> ={res, glob Ob})=> //; sim.
+  + by conseq (: _ ==> ={res, glob Ob})=> //; sim.
+  by auto=> /> l0 /supp_dinter /#.
+  qed.
 end section.
